Tried to put safety back in.

Java/src/Java/Logic/Traces.v
@@ -24,7 +24,7 @@ Proof.
 Qed.
 
 Inductive trace : Type :=
-  | t_end   : trace
+  | t_end   : Lang.stack -> heap -> NS.t -> trace
   | t_fail  : trace
   | t_send  : stptr -> val -> heap -> trace -> trace
   | t_recv  : stptr -> (ptr -> heap -> trace) -> trace
@@ -32,23 +32,9 @@ Inductive trace : Type :=
   | t_tau : Lang.stack -> heap -> NS.t -> trace -> trace
   .
   
-Fixpoint trace_wf (tr : trace) : Prop :=
-	match tr with
-		| t_end => True
-		| t_fail => True
-		| t_send _ _ _ (t_tau _ _ _ tr') => trace_wf tr'
-		| t_recv _ ftr => forall v h, match ftr v h with
-							            | t_tau _ _ _ tr' => trace_wf tr'
-							            | _ => False
-							          end
-		| t_start _ _ tr' => trace_wf tr'
-		| t_tau _ _ _ tr' => trace_wf tr'
-		| _ => False
-	end.
-
 Fixpoint trace_safe (tr : trace) : Prop :=
 	match tr with
-		| t_end => True
+		| t_end _ _ _ => True
 		| t_fail => False
 		| t_send _ _ _ tr' => trace_safe tr'
 		| t_recv _ ftr => forall v h, trace_safe (ftr v h)
@@ -58,7 +44,7 @@ Fixpoint trace_safe (tr : trace) : Prop :=
 
 Fixpoint fail_trace (tr : trace) : Prop :=
 	match tr with
-		| t_end => False
+		| t_end _ _ _ => False
 		| t_fail => True
 		| t_send _ _ _ tr' => fail_trace tr'
 		| t_recv _ ftr => exists v h, fail_trace (ftr v h)
