Java/src/Java/Semantics/SemCmd.v
@@ -14,7 +14,7 @@ Section Compatability.
 
   Program Fixpoint Comp (Pr : Prog_wf) (n : nat) (pr : STs) (tr : trace) (Q : psasn) : Prop :=
     match tr with 
-      | t_end => False
+      | t_end s h _ => Q s pr Pr (n - 1) h
       | t_fail => False
       | t_send x v h tr' => match (find x pr) with
           | Some (st_send z P T) =>  P (stack_add z v (stack_empty _)) Pr n h /\ Comp Pr (n - 1) (add x (subst_ST z v T) pr) tr' Q
@@ -30,10 +30,7 @@ Section Compatability.
                (fun s => mk_pasn (fun pr' Pr n _ => (forall c', In c' pr' -> MapsTo c' st_end pr') /\ 
           			                               forall m, m <= n -> forall Pr', Prog_wf_sub Pr Pr' ->
           			                                  Comp Pr' m (add x (dual T) pr) tr'' Q) _ _ _ _)
-      | t_tau s h _ tr' => match tr' with
-                         | t_end => Q s pr Pr n h 
-                         | _     => Comp Pr (n - 1) pr tr' Q
-                         end
+      | t_tau _ _ _ tr' => Comp Pr (n - 1) pr tr' Q
     end.
     Next Obligation.
 	  split; [|assumption].
@@ -62,7 +59,6 @@ Section Compatability.
       eapply IHtr1; [| apply H].
       intros. simpl in *. destruct H0; split; [assumption|].
       intros; eapply IHtr2. eapply HQQ'. apply H1. assumption. assumption.
-    - destruct tr; try eapply HQQ'; try eassumption; try eapply IHtr; eassumption.
   Qed.
 (*
   Lemma Comp_split : forall Pr n pr tr (P Q : nat -> STs -> Prop), Comp Pr n pr tr P -> Comp Pr n pr tr Q -> Comp Pr n pr tr (fun n pr' => P n pr' /\ Q n pr').
@@ -116,11 +112,11 @@ End Compatability.
 
 Section Commands.
 
-  Definition semCmdType := Prog_wf -> stack -> heap -> NS.t -> trace -> Type.
+  Definition semCmdType := Prog_wf -> stack -> heap -> NS.t -> trace -> Prop.
   Definition safe (c : semCmdType) Pr s h cl := forall tr, c Pr s h cl tr -> trace_safe tr.
 
-  Inductive frame_trace (frame : heap) : trace -> trace -> Type :=
-  	| ft_end : frame_trace frame t_end t_end
+  Inductive frame_trace (frame : heap) : trace -> trace -> Prop :=
+  	| ft_end s big cl h : sa_mul h frame big -> frame_trace frame (t_end s h cl) (t_end s big cl)
   	| ft_fail tr : frame_trace frame t_fail tr
   	| ft_tau tr tr' s big cl h : frame_trace frame tr tr' ->
   	                 sa_mul h frame big -> frame_trace frame (t_tau s h cl tr) (t_tau s big cl tr')
@@ -129,11 +125,12 @@ Section Commands.
   	| ft_recv f g c : (forall x h, frame_trace frame (f x h) (g x h)) -> frame_trace frame (t_recv c f) (t_recv c g)
   	| ft_start c tr tr' tr'' : frame_trace frame tr tr' -> frame_trace frame (t_start c tr'' tr) (t_start c tr'' tr').
 
-  Definition frame_property (c : semCmdType) : Type :=
+  Definition frame_property (c : semCmdType) : Prop :=
     forall Pr s (big frame h : heap) cl tr
       (HFrame : @sa_mul heap HeapSepAlgOps h frame big) 
+      (HSafe : safe c Pr s h cl)
       (HSem   : c Pr s big cl tr),
-      sigT (fun tr' => (frame_trace frame tr' tr * c Pr s h cl tr')%type).
+      exists tr', frame_trace frame tr' tr /\ c Pr s h cl tr'.
 (*
   Definition frame_property (c : semCmdType) :=
     forall Pr s s' (big big' frame h : heap) cl cl' tr
@@ -144,7 +141,6 @@ Section Commands.
 *)
   Record semCmd := {
     cmd_rel   :> Prog_wf -> stack -> heap -> NS.t -> trace -> Prop;
-    cmd_zero  :  forall Pr s h cl, ~(cmd_rel Pr s h cl t_end);
     cmd_frame : frame_property cmd_rel
   }.
   Print semCmd.
@@ -175,78 +171,120 @@ Section Commands.
 *)
 
   Inductive skip_sem : semCmdType :=
-  | s_ok : forall Pr s h cl, skip_sem Pr s h cl (t_tau s h cl t_end).
-  Program Definition skip_cmd := @Build_semCmd skip_sem _ _.
-  Next Obligation.
+  | s_ok : forall Pr s h cl, skip_sem Pr s h cl (t_end s h cl).
+  Program Definition skip_cmd := @Build_semCmd skip_sem _.
+(*  Next Obligation.
     intros H. inversion H.
-  Qed.
+  Qed.*)
   Next Obligation.
 	unfold frame_property.
 	intros. inversion HSem; subst.
-	admit.
+	exists (t_end s h cl).
+	split; constructor; assumption.
   Qed.
 
   (* Seq *)
-
-  Inductive trace_append_cmd (Pr : Prog_wf) (c : semCmd) : trace -> trace -> Type :=
+ 
+  Inductive trace_append_cmd (Pr : Prog_wf) (c : semCmd) : trace -> trace -> Prop :=
     | ta_fail : trace_append_cmd Pr c t_fail t_fail
   	| ta_send p v h tr tr' : trace_append_cmd Pr c tr tr' ->
   	                         trace_append_cmd Pr c (t_send p v h tr) (t_send p v h tr')
   	| ta_recv p f g: (forall v h, trace_append_cmd Pr c (f v h) (g v h)) ->
   	                              trace_append_cmd Pr c (t_recv p f) (t_recv p g)
-  	| ta_bc s h tr cl : c Pr s h cl tr -> trace_append_cmd Pr c (t_tau s h cl t_end) (t_tau s h cl tr)
+  	| ta_end s h tr cl : c Pr s h cl tr -> trace_append_cmd Pr c (t_end s h cl) (t_tau s h cl tr)
   	| ta_tau s h tr tr' cl : trace_append_cmd Pr c tr tr' -> 
-  	                         trace_append_cmd Pr c (t_tau s h cl tr) (t_tau s h cl tr').
-  
+  	                         trace_append_cmd Pr c (t_tau s h cl tr) (t_tau s h cl tr')
+    | ta_start p tr tr' tr'' : trace_append_cmd Pr c tr' tr'' -> 
+                               trace_append_cmd Pr c (t_start p tr tr') (t_start p tr tr'').                
+    
+ 
     Lemma trace_append_cmd_frame_trace Pr c tr tr' tr'' frame
     	(Hc : trace_append_cmd Pr c tr tr') (HFrame : frame_trace frame tr'' tr) :
-    	sigT (fun tr''' => (trace_append_cmd Pr c tr'' tr''' * frame_trace frame tr''' tr')%type).
+    	exists tr''', trace_append_cmd Pr c tr'' tr''' /\ frame_trace frame tr''' tr'.
     Proof with eauto.
+ 	  admit.
+ 	  (*
       generalize dependent tr'. induction HFrame; intros.
       + inversion Hc.
       + exists t_fail; try repeat constructor.
       + inversion Hc; subst.
         inversion HFrame; subst.
+        inversion Hc; subst; [|inversion H1].
+        admit. inversion H1.
         edestruct (@cmd_frame c) as [tr2 [HFrame2 HSem2]]...
+        inversion Hc.
         exists (t_tau s h cl tr2).
         split.
         constructor; assumption.
         constructor; assumption.
         exists (t_tau s h cl t_fail). split; try repeat constructor. assumption.
-        specialize (IHHFrame _ X).
+        specialize (IHHFrame _ H5).
         destruct IHHFrame as [tr''' [H1 H2]].
         exists (t_tau s h cl tr'''). 
         split; constructor; assumption.
       + inversion Hc; subst.
-        specialize (IHHFrame _ X).
+        specialize (IHHFrame _ H5).
         destruct IHHFrame as [tr''' [H1 H2]].
         exists (t_send x v h tr''').
         split; constructor; assumption.
       + inversion Hc; subst.
-        exists (t_recv c0 (fun x h => match X x h (g0 x h) (X0 x h) with existT w P => w end)).
-	    split; constructor; intros.
-	    - destruct (X v h (g0 v h) (X0 v h)) as [tr2 [H _]]; apply H.
-	    - destruct (X x h (g0 x h) (X0 x h)) as [tr2 [_ H]]; apply H.
+     assert (forall x h, 
+     exists tr''' : trace,
+       trace_append_cmd Pr c (f x h) tr''' /\ frame_trace frame tr''' (g0 x h)).
+       intros. apply H0. apply H4. clear H0.
+       
+       Require Import ChoiceFacts.
+       Axiom AC_fun : FunctionalChoice.
+       assert (forall (x : ptr), exists tr''' : heap -> trace, forall h : heap,
+       trace_append_cmd Pr c (f x h) (tr''' h) /\
+       frame_trace frame (tr''' h) (g0 x h)).
+       intros. specialize (H1 x). apply AC_fun in H1.
+       apply H1. clear H1.
+       apply AC_fun in H0. destruct H0.
+       exists (t_recv c0 x). 
+       split; constructor; intros; firstorder.
       + inversion Hc.
+*)
    Qed.
 
 
     Inductive seq_sem (c1 c2 : semCmd) : semCmdType :=
     | seq_ok : forall Pr s h cl tr tr',
     	c1 Pr s h cl tr ->
-    	trace_append_cmd Pr c2 tr tr' ->
+     	trace_append_cmd Pr c2 tr tr' ->
     	seq_sem c1 c2 Pr s h cl tr'.
-  Program Definition seq_cmd c1 c2 := @Build_semCmd (seq_sem c1 c2) _ _.
-  Next Obligation.
-	intros H; inversion H; subst. inversion X.
-  Qed.
+  Program Definition seq_cmd c1 c2 := @Build_semCmd (seq_sem c1 c2) _.
+(*  Next Obligation.
+	intros H; inversion H; subst. inversion H1.
+  Qed.*)
   Next Obligation with eauto using seq_sem.
     unfold frame_property; intros.
     inversion HSem; subst.
-    edestruct (@cmd_frame c1) as [tr1 [HFrame1 Hsem1]]...
-            
-    pose proof (trace_append_cmd_frame_trace X HFrame1).
-    destruct X0 as [tr' [H1 H2]].
+    edestruct (@cmd_frame c1) as [tr1 [HFrame1 Hsem1]]... 
+    intros tr' Hc.
+    + intros tr' Hc. 
+      clear -HSafe Hc.
+      destruct tr'; simpl in *; try apply I.
+      - specialize (HSafe t_fail). apply HSafe. 
+        eapply seq_ok; [eassumption|]. constructor.
+      - unfold safe in HSafe. 
+	    assert (exists tr'', trace_append_cmd Pr c2 tr' tr'') by admit.
+	    destruct H as [tr'' H].
+	    specialize (HSafe (t_send s0 v h0 tr'')).
+	    simpl in HSafe. 
+	    assert (trace_append_cmd Pr c2 (t_send s0 v h0 tr') (t_send s0 v h0 tr'')).
+	    constructor. assumption.
+	    pose proof (seq_ok Hc H0).
+	    specialize (HSafe H1).
+	    
+	    apply HSafe.
+      unfold safe in HSafe.
+      
+      specialize (H0 Htrace).
+    apply HSafe.
+    eapply seq_ok. eassumption.
+    pose proof (trace_append_cmd_frame_trace H0 HFrame1).
+    destruct H1 as [tr' [H1 H2]].
     exists tr'. split; [assumption|].
     eapply seq_ok; eassumption.
   Qed.
@@ -259,19 +297,19 @@ Section Commands.
    | nondetR   : forall Pr s h tr cl,
       c2 Pr s h cl tr ->
       nondet_sem c1 c2 Pr s h cl tr.
-  Program Definition nondet_cmd c1 c2 := @Build_semCmd (nondet_sem c1 c2) _ _.
-  Next Obligation.
+  Program Definition nondet_cmd c1 c2 := @Build_semCmd (nondet_sem c1 c2) _.
+(*  Next Obligation.
     intros H; inversion H; subst;
     apply cmd_zero in H0; assumption.
-  Qed.
+  Qed.*)
   Next Obligation with eauto using nondet_sem.
 	intros Pr s big frame h cl tr HFrame HSem.
 	inversion HSem; subst.
 	+ edestruct (@cmd_frame c1)...
-	  exists x. destruct p as [H1 H2]. split; [assumption|].
+	  exists x. destruct H0 as [H1 H2]. split; [assumption|].
 	  apply nondetL; assumption.
 	+ edestruct (@cmd_frame c2)...
-	  exists x; destruct p as [H1 H2]; split; [assumption|].
+	  exists x; destruct H0 as [H1 H2]; split; [assumption|].
 	  apply nondetR; assumption.
   Qed.
 
@@ -279,23 +317,23 @@ Section Commands.
 
   Inductive kleene_sem (c : semCmd) : semCmdType :=
   | kleene_emp       : forall Pr s h cl,
-      kleene_sem c Pr s h cl (t_tau s h cl t_end)
+      kleene_sem c Pr s h cl (t_end s h cl)
   | kleene_step_ok   : forall Pr s h tr tr1 cl,
       c Pr s h cl tr ->
       trace_append_cmd Pr c tr tr1 ->
       kleene_sem c Pr s h cl tr1.
-  Program Definition kleene_cmd c := @Build_semCmd (kleene_sem c) _ _.
-  Next Obligation.
-	intros H; inversion H; subst. inversion X. 
-  Qed.
+  Program Definition kleene_cmd c := @Build_semCmd (kleene_sem c) _.
+(*  Next Obligation.
+	intros H; inversion H; subst. inversion H1. 
+  Qed.*)
   Next Obligation with eauto using kleene_sem.
     unfold frame_property; intros.
     generalize dependent h. induction HSem; intros.
-    + exists (t_tau s h0 cl t_end).
+    + exists (t_end s h0 cl).
       split; try repeat constructor; assumption.
     + edestruct (@cmd_frame c) as [tr2 [HFrame1 Hsem1]]...            
-      pose proof (trace_append_cmd_frame_trace t HFrame1).
-      destruct X as [tr' [H1 H2]].
+      pose proof (trace_append_cmd_frame_trace H0 HFrame1).
+      destruct H1 as [tr' [H1 H2]].
       exists tr'. split; [assumption|].
       eapply kleene_step_ok; eassumption.
   Qed.
@@ -305,15 +343,15 @@ Section Commands.
      a check holds and loops otherwise, this way allowing to encode if/while
      using nondeterministic choice/Kleene star *)
   Inductive assume_sem (p : vlogic) : semCmdType :=
-  | assume_ok : forall Pr s h cl, p s -> assume_sem p Pr s h cl (t_tau s h cl t_end).
-  Program Definition assume_cmd P := @Build_semCmd (assume_sem P) _ _.
-  Next Obligation.
+  | assume_ok : forall Pr s h cl, p s -> assume_sem p Pr s h cl (t_end s h cl).
+  Program Definition assume_cmd P := @Build_semCmd (assume_sem P) _.
+(*  Next Obligation.
     intros H; inversion H.
-  Qed.
+  Qed.*)
   Next Obligation.
     unfold frame_property; intros.
     induction HSem.
-    exists (t_tau s h cl t_end).
+    exists (t_end s h cl).
     split; try repeat constructor; assumption.
   Qed.
 
@@ -327,17 +365,17 @@ Section Commands.
 *)
   Inductive assert_sem (p : vlogic) : semCmdType :=
   | assert_ok   : forall Pr s h cl (HP : p s),
-    assert_sem p Pr s h cl (t_tau s h cl t_end)
+    assert_sem p Pr s h cl (t_end s h cl)
   | assert_fail : forall Pr s h cl (HNP : ~p s),
     assert_sem p Pr s h cl t_fail.
-  Program Definition assert_cmd p := @Build_semCmd (assert_sem p) _ _.
-  Next Obligation.
+  Program Definition assert_cmd p := @Build_semCmd (assert_sem p) _.
+(*  Next Obligation.
     intros H; inversion H.
-  Qed.
+  Qed.*)
   Next Obligation with eauto using assert_sem.
     unfold frame_property; intros.
     inversion HSem; subst...
-    + exists (t_tau s h cl t_end); split; try repeat constructor; assumption.
+    + exists (t_end s h cl); split; try repeat constructor; assumption.
     + exists t_fail; split; try repeat constructor; assumption.
   Qed.
 
